Separate definitions from theories

KeyManagement/AdversaryUniverse.v
@@ -13,118 +13,151 @@ Require Import
         Keys
         Automation
         Tactics
-        CipherTheory
-        MessagesTheory
-        UsersTheory
-        KeysTheory
+        RealWorld
 .
-
-Require IdealWorld
-        RealWorld.
 
 Set Implicit Arguments.
 
-Lemma accepted_safe_msg_pattern_msg_filter_true :
-  forall {t} (msg : RealWorld.crypto t) honestk cs msg_to pat,
-    RealWorld.msg_pattern_safe honestk pat
-    -> RealWorld.msg_accepted_by_pattern cs msg_to pat msg
-    -> RealWorld.msg_honestly_signed honestk cs msg = true
-    /\ RealWorld.msg_to_this_user cs msg_to msg = true.
-Proof.
-  intros.
-  destruct msg;
-    repeat match goal with
-           | [ H : RealWorld.msg_pattern_safe _ _ |- _] => invert H
-           | [ H : RealWorld.msg_accepted_by_pattern _ _ _ _ |- _] => invert H
-           end;
-    unfold RealWorld.msg_honestly_signed, RealWorld.msg_to_this_user;
-    simpl; context_map_rewrites; unfold RealWorld.cipher_to_user;
-      destruct (msg_to0 ==n msg_to0); subst; try contradiction;
-      rewrite <- RealWorld.honest_key_honest_keyb; auto.
-Qed.
+Section Cleanliness.
 
-Lemma accepted_safe_msg_pattern_honestly_signed :
-  forall {t} (msg : RealWorld.crypto t) honestk cs msg_to pat,
-    RealWorld.msg_pattern_safe honestk pat
-    -> RealWorld.msg_accepted_by_pattern cs msg_to pat msg
-    -> RealWorld.msg_honestly_signed honestk cs msg = true.
-Proof.
-  intros;
-    pose proof (accepted_safe_msg_pattern_msg_filter_true H H0); split_ands; assumption.
-Qed.
+  Variable honestk : key_perms.
 
-Lemma accepted_safe_msg_pattern_to_this_user :
-  forall {t} (msg : RealWorld.crypto t) honestk cs msg_to pat,
-    RealWorld.msg_pattern_safe honestk pat
-    -> RealWorld.msg_accepted_by_pattern cs msg_to pat msg
-    -> RealWorld.msg_to_this_user cs msg_to msg = true.
-Proof.
-  intros;
-    pose proof (accepted_safe_msg_pattern_msg_filter_true H H0); split_ands; assumption.
-Qed.
+  (******************** KEYS CLEANING ************************)
 
-Hint Resolve
-     accepted_safe_msg_pattern_honestly_signed
-     accepted_safe_msg_pattern_to_this_user.
-
-
-Section StripAdv.
-  Import RealWorld.
-
-  Definition clean_adv_msgs (honestk : key_perms) (cs : ciphers) (msgs : queued_messages) :=
-    List.filter (fun sigM => match sigM with 
-                          | existT _ _ msg => msg_honestly_signed honestk cs msg
-                          end) msgs.
-
-  Definition clean_adv {B} (adv : user_data B) (honestk : key_perms) (cs : ciphers) (b : B) :=
-    {| key_heap := clean_key_permissions honestk adv.(key_heap)
-     ; protocol := Return b
-     (* ; msg_heap := clean_messages honestk cs None adv.(from_ids) adv.(msg_heap) *)
-     ; msg_heap := clean_adv_msgs honestk cs adv.(msg_heap)
-     ; c_heap   := []
-     ; from_nons := []
-     ; sent_nons := []
-     ; cur_nonce := adv.(cur_nonce) |}.
-
-  Definition strip_adversary_univ {A B} (U__r : universe A B) (b : B) : universe A B :=
-    let honestk := findUserKeys U__r.(users)
-    in {| users       := clean_users honestk U__r.(all_ciphers) U__r.(users)
-        ; adversary   := clean_adv U__r.(adversary) honestk U__r.(all_ciphers) b
-        ; all_ciphers := clean_ciphers honestk U__r.(all_ciphers)
-        ; all_keys    := clean_keys honestk U__r.(all_keys)
-       |}.
-
-  Definition strip_adversary {A B} (U__r : universe A B) : simpl_universe A :=
-    let honestk := findUserKeys U__r.(users)
-    in {| s_users       := clean_users honestk U__r.(all_ciphers) U__r.(users)
-        ; s_all_ciphers := clean_ciphers honestk U__r.(all_ciphers)
-        ; s_all_keys    := clean_keys honestk U__r.(all_keys)
-       |}.
-
-  Definition strip_adversary_simpl {A} (U__r : simpl_universe A) : simpl_universe A :=
-    let honestk := findUserKeys U__r.(s_users)
-    in {| s_users       := clean_users honestk U__r.(s_all_ciphers) U__r.(s_users)
-        ; s_all_ciphers := clean_ciphers honestk U__r.(s_all_ciphers)
-        ; s_all_keys    := clean_keys honestk U__r.(s_all_keys)
-       |}.
-
-  Definition strip_action (honestk : key_perms) (cs : ciphers) (act : action) :=
-    match act with
-    | Input msg pat froms     => Input msg pat froms
-    | Output msg msg_from msg_to sents => Output msg msg_from msg_to sents
+  Definition honest_key_filter_fn (k_id : key_identifier) (k : key) :=
+    match honestk $? k_id with
+    | Some true => true
+    | _ => false
     end.
 
-  Definition strip_label (honestk : key_perms) (cs : ciphers) (lbl : label) :=
-    match lbl with
-    | Silent => Silent
-    | Action a => Action (strip_action honestk cs a)
+  Definition clean_keys :=
+    filter honest_key_filter_fn.
+
+  Definition honest_perm_filter_fn (k_id : key_identifier) (kp : bool) :=
+    match honestk $? k_id with
+    | Some true => true
+    | _ => false
     end.
 
-  Lemma peel_strip_univ_eq_strip_adv :
-    forall A B (U : universe A B) b,
-      peel_adv (strip_adversary_univ U b) = strip_adversary U.
-  Proof.
-    unfold peel_adv, strip_adversary, strip_adversary_univ; trivial.
-  Qed.
+  Definition clean_key_permissions :=
+    filter honest_perm_filter_fn.
 
-End StripAdv.
+  (******************** CIPHERS CLEANING *********************)
+
+  Definition honest_cipher_filter_fn (c_id : cipher_id) (c : cipher) :=
+    cipher_honestly_signed honestk c.
+
+  Definition clean_ciphers (cs : ciphers) :=
+    filter honest_cipher_filter_fn cs.
+
+  (******************** MESSAGES CLEANING ********************)
+
+  Section Messages.
+  
+    Variable cs : ciphers.
+
+    Definition msg_nonce_ok {t} (froms : recv_nonces) (msg : crypto t) : option recv_nonces :=
+      match msg with
+      | Content _ => Some froms
+      | SignedCiphertext c_id =>
+        match cs $? c_id with
+        | None => None
+        | Some c =>
+          match count_occ msg_seq_eq froms (cipher_nonce c) with
+          | 0 => Some (cipher_nonce c :: froms)
+          | _ => None
+          end
+        end
+      end.
+
+    Definition msg_filter
+               (to_user_id : option user_id) 
+               (fld_param : queued_messages * recv_nonces)
+               (sigM : { t & crypto t } ) : queued_messages * recv_nonces :=
+      match sigM with
+      | existT _ _ msg =>
+        if msg_signed_addressed honestk cs to_user_id msg
+        then match msg_nonce_ok (snd fld_param) msg with
+             | None => fld_param
+             | Some froms => (fst fld_param ++ [sigM], froms)
+             end
+        else fld_param
+      end.
+
+    Definition clean_messages' (to_usr_id : option user_id) (froms : recv_nonces) (acc msgs : queued_messages) :=
+      List.fold_left (msg_filter to_usr_id) msgs (acc, froms).
+    
+    Definition clean_messages (to_usr_id : option user_id) (froms : recv_nonces) (msgs : queued_messages) :=
+      fst (clean_messages' to_usr_id froms [] msgs).
+    
+  End Messages.
+
+  (******************** USERS CLEANING ***********************)
+
+  Definition clean_users {A} (cs : ciphers) (usrs : honest_users A) :=
+    mapi (fun u_id u_d => {| key_heap  := clean_key_permissions u_d.(key_heap)
+                        ; protocol  := u_d.(protocol)
+                        ; msg_heap  := clean_messages cs (Some u_id) u_d.(from_nons) u_d.(msg_heap)
+                        ; c_heap    := u_d.(c_heap)
+                        ; from_nons := u_d.(from_nons)
+                        ; sent_nons := u_d.(sent_nons)
+                        ; cur_nonce := u_d.(cur_nonce) |}) usrs.
+
+End Cleanliness.
+
+(******************** UNIVERSE CLEANING ***********************)
+
+Definition clean_adv_msgs (honestk : key_perms) (cs : ciphers) (msgs : queued_messages) :=
+  List.filter (fun sigM => match sigM with 
+                        | existT _ _ msg => msg_honestly_signed honestk cs msg
+                        end) msgs.
+
+Definition clean_adv {B} (adv : user_data B) (honestk : key_perms) (cs : ciphers) (b : B) :=
+  {| key_heap := clean_key_permissions honestk adv.(key_heap)
+   ; protocol := Return b
+   ; msg_heap := clean_adv_msgs honestk cs adv.(msg_heap)
+   ; c_heap   := []
+   ; from_nons := []
+   ; sent_nons := []
+   ; cur_nonce := adv.(cur_nonce) |}.
+
+Definition strip_adversary_univ {A B} (U__r : universe A B) (b : B) : universe A B :=
+  let honestk := findUserKeys U__r.(users)
+  in {| users       := clean_users honestk U__r.(all_ciphers) U__r.(users)
+      ; adversary   := clean_adv U__r.(adversary) honestk U__r.(all_ciphers) b
+      ; all_ciphers := clean_ciphers honestk U__r.(all_ciphers)
+      ; all_keys    := clean_keys honestk U__r.(all_keys)
+     |}.
+
+Definition strip_adversary {A B} (U__r : universe A B) : simpl_universe A :=
+  let honestk := findUserKeys U__r.(users)
+  in {| s_users       := clean_users honestk U__r.(all_ciphers) U__r.(users)
+      ; s_all_ciphers := clean_ciphers honestk U__r.(all_ciphers)
+      ; s_all_keys    := clean_keys honestk U__r.(all_keys)
+     |}.
+
+Definition strip_adversary_simpl {A} (U__r : simpl_universe A) : simpl_universe A :=
+  let honestk := findUserKeys U__r.(s_users)
+  in {| s_users       := clean_users honestk U__r.(s_all_ciphers) U__r.(s_users)
+      ; s_all_ciphers := clean_ciphers honestk U__r.(s_all_ciphers)
+      ; s_all_keys    := clean_keys honestk U__r.(s_all_keys)
+     |}.
+
+Definition strip_action (honestk : key_perms) (cs : ciphers) (act : action) :=
+  match act with
+  | Input msg pat froms     => Input msg pat froms
+  | Output msg msg_from msg_to sents => Output msg msg_from msg_to sents
+  end.
+
+Definition strip_label (honestk : key_perms) (cs : ciphers) (lbl : label) :=
+  match lbl with
+  | Silent => Silent
+  | Action a => Action (strip_action honestk cs a)
+  end.
+
+Lemma peel_strip_univ_eq_strip_adv :
+  forall A B (U : universe A B) b,
+    peel_adv (strip_adversary_univ U b) = strip_adversary U.
+Proof.
+  unfold peel_adv, strip_adversary, strip_adversary_univ; trivial.
+Qed.
