KeyManagement/KeysTheory.v
@@ -14,44 +14,29 @@ Require Import
         Automation
         Tactics
         RealWorld
-        CipherTheory.
+        AdversaryUniverse.
 
 Set Implicit Arguments.
-
-(******************** KEYS CLEANING ***********************
- **********************************************************
- *
- * Function to clean keys and lemmas about it.
- *)
 
 Section CleanKeys.
   Import RealWorld.
 
   Variable honestk : key_perms.
 
-  Definition honest_key_filter_fn (k_id : key_identifier) (k : key) :=
-    match honestk $? k_id with
-    | Some true => true
-    | _ => false
-    end.
-
-  Definition clean_keys :=
-    filter honest_key_filter_fn.
-
   Lemma honest_key_filter_fn_proper :
-    Proper (eq  ==>  eq  ==>  eq) honest_key_filter_fn.
+    Proper (eq  ==>  eq  ==>  eq) (honest_key_filter_fn honestk).
   Proof.
     solve_proper.
   Qed.
 
   Lemma honest_key_filter_fn_filter_proper :
-    Proper (eq  ==>  eq  ==>  eq  ==>  eq) (fun k v m => if honest_key_filter_fn k v then m $+ (k,v) else m).
+    Proper (eq  ==>  eq  ==>  eq  ==>  eq) (fun k v m => if honest_key_filter_fn honestk k v then m $+ (k,v) else m).
   Proof.
     solve_proper.
   Qed.
 
   Lemma honest_key_filter_fn_filter_transpose :
-    transpose_neqkey eq (fun k v m => if honest_key_filter_fn k v then m $+ (k,v) else m).
+    transpose_neqkey eq (fun k v m => if honest_key_filter_fn honestk k v then m $+ (k,v) else m).
   Proof.
     unfold transpose_neqkey; intros.
     unfold honest_key_filter_fn.
@@ -61,15 +46,15 @@ Section CleanKeys.
   Qed.
 
   Lemma honest_key_filter_fn_filter_proper_Equal :
-    Proper (eq  ==>  eq  ==>  Equal  ==>  Equal) (fun k v m => if honest_key_filter_fn k v then m $+ (k,v) else m).
+    Proper (eq  ==>  eq  ==>  Equal  ==>  Equal) (fun k v m => if honest_key_filter_fn honestk k v then m $+ (k,v) else m).
   Proof.
     unfold Equal, Proper, respectful; intros; subst.
-    destruct (honest_key_filter_fn y y0); eauto.
+    destruct (honest_key_filter_fn honestk y y0); eauto.
     destruct (y ==n y2); subst; clean_map_lookups; auto.
   Qed.
 
   Lemma honest_key_filter_fn_filter_transpose_Equal :
-    transpose_neqkey Equal (fun k v m => if honest_key_filter_fn k v then m $+ (k,v) else m).
+    transpose_neqkey Equal (fun k v m => if honest_key_filter_fn honestk k v then m $+ (k,v) else m).
   Proof.
     unfold transpose_neqkey, Equal; intros.
     unfold honest_key_filter_fn.
@@ -85,9 +70,9 @@ Section CleanKeys.
 
   Lemma clean_keys_inv :
     forall k_id k ks,
-      clean_keys ks $? k_id = Some k
+      clean_keys honestk ks $? k_id = Some k
       -> ks $? k_id = Some k
-      /\ honest_key_filter_fn k_id k = true.
+      /\ honest_key_filter_fn honestk k_id k = true.
   Proof.
     unfold clean_keys; intros until ks.
     rewrite <- !find_mapsto_iff.
@@ -96,27 +81,27 @@ Section CleanKeys.
 
   Lemma clean_keys_inv' :
     forall k_id k ks,
-      clean_keys ks $? k_id = None
+      clean_keys honestk ks $? k_id = None
       -> ks $? k_id = Some k
-      -> honest_key_filter_fn k_id k = false.
+      -> honest_key_filter_fn honestk k_id k = false.
   Proof.
     induction ks using P.map_induction_bis; intros; Equal_eq; clean_map_lookups; eauto.
 
     destruct (x ==n k_id); subst; clean_map_lookups; eauto.
     - unfold clean_keys,filter in H0; rewrite fold_add in H0; eauto.
-      cases (honest_key_filter_fn k_id k); clean_map_lookups; try discriminate; trivial.
+      cases (honest_key_filter_fn honestk k_id k); clean_map_lookups; try discriminate; trivial.
     - eapply IHks; eauto.
       unfold clean_keys, filter in H0.
       rewrite fold_add in H0; eauto.
-      cases (honest_key_filter_fn x e); eauto.
+      cases (honest_key_filter_fn honestk x e); eauto.
       clean_map_lookups; eauto.
   Qed.
 
   Lemma clean_keys_keeps_honest_key :
     forall k_id k ks,
         ks $? k_id = Some k
-      -> honest_key_filter_fn k_id k = true
-      -> clean_keys ks $? k_id = Some k.
+      -> honest_key_filter_fn honestk k_id k = true
+      -> clean_keys honestk ks $? k_id = Some k.
   Proof.
     unfold clean_keys; intros.
     rewrite <- !find_mapsto_iff.
@@ -127,14 +112,14 @@ Section CleanKeys.
   Lemma clean_keys_drops_dishonest_key :
     forall k_id k ks,
         ks $? k_id = Some k
-      -> honest_key_filter_fn k_id k = false
-      -> clean_keys ks $? k_id = None.
+      -> honest_key_filter_fn honestk k_id k = false
+      -> clean_keys honestk ks $? k_id = None.
   Proof.
     unfold clean_keys; intros.
     rewrite <- not_find_in_iff.
     unfold not; intros.
     rewrite in_find_iff in H1.
-    cases (filter honest_key_filter_fn ks $? k_id); try contradiction.
+    cases (filter (honest_key_filter_fn honestk) ks $? k_id); try contradiction.
     rewrite <- find_mapsto_iff in Heq.
     rewrite filter_iff in Heq; eauto.
     split_ands.
@@ -146,49 +131,40 @@ Section CleanKeys.
   Lemma clean_keys_adds_no_keys :
     forall k_id ks,
         ks $? k_id = None
-      -> clean_keys ks $? k_id = None.
+      -> clean_keys honestk ks $? k_id = None.
   Proof.
     induction ks using P.map_induction_bis; intros; Equal_eq; eauto.
     unfold clean_keys, filter; rewrite fold_add; eauto.
     destruct (x ==n k_id); subst; clean_map_lookups.
-    destruct (honest_key_filter_fn x e); eauto.
+    destruct (honest_key_filter_fn honestk x e); eauto.
     clean_map_lookups; eauto.
   Qed.
 
   Lemma clean_keys_idempotent :
     forall ks,
-      clean_keys (clean_keys ks) = clean_keys ks.
+      clean_keys honestk (clean_keys honestk ks) = clean_keys honestk ks.
   Proof.
     intros.
     apply map_eq_Equal; unfold Equal; intros.
-    cases (clean_keys ks $? y); eauto using clean_keys_adds_no_keys.
+    cases (clean_keys honestk ks $? y); eauto using clean_keys_adds_no_keys.
     eapply clean_keys_keeps_honest_key; auto.
     apply clean_keys_inv in Heq; split_ands; auto.
   Qed.
 
-  Definition honest_perm_filter_fn (k_id : key_identifier) (kp : bool) :=
-    match honestk $? k_id with
-    | Some true => true
-    | _ => false
-    end.
-
-  Definition clean_key_permissions :=
-    filter honest_perm_filter_fn.
-
   Lemma honest_perm_filter_fn_proper :
-    Proper (eq  ==>  eq  ==>  eq) honest_perm_filter_fn.
+    Proper (eq  ==>  eq  ==>  eq) (honest_perm_filter_fn honestk).
   Proof.
     solve_proper.
   Qed.
 
   Lemma honest_perm_filter_fn_filter_proper :
-    Proper (eq  ==>  eq  ==>  eq  ==>  eq) (fun k v m => if honest_perm_filter_fn k v then m $+ (k,v) else m).
+    Proper (eq  ==>  eq  ==>  eq  ==>  eq) (fun k v m => if honest_perm_filter_fn honestk  k v then m $+ (k,v) else m).
   Proof.
     solve_proper.
   Qed.
 
   Lemma honest_perm_filter_fn_filter_transpose :
-    transpose_neqkey eq (fun k v m => if honest_perm_filter_fn k v then m $+ (k,v) else m).
+    transpose_neqkey eq (fun k v m => if honest_perm_filter_fn honestk k v then m $+ (k,v) else m).
   Proof.
     unfold transpose_neqkey; intros.
     unfold honest_perm_filter_fn.
@@ -198,15 +174,15 @@ Section CleanKeys.
   Qed.
 
   Lemma honest_perm_filter_fn_filter_proper_Equal :
-    Proper (eq  ==>  eq  ==>  Equal  ==>  Equal) (fun k v m => if honest_perm_filter_fn k v then m $+ (k,v) else m).
+    Proper (eq  ==>  eq  ==>  Equal  ==>  Equal) (fun k v m => if honest_perm_filter_fn honestk k v then m $+ (k,v) else m).
   Proof.
     unfold Equal, Proper, respectful; intros; subst.
-    destruct (honest_perm_filter_fn y y0); eauto.
+    destruct (honest_perm_filter_fn honestk y y0); eauto.
     destruct (y ==n y2); subst; clean_map_lookups; auto.
   Qed.
 
   Lemma honest_perm_filter_fn_filter_transpose_Equal :
-    transpose_neqkey Equal (fun k v m => if honest_perm_filter_fn k v then m $+ (k,v) else m).
+    transpose_neqkey Equal (fun k v m => if honest_perm_filter_fn honestk k v then m $+ (k,v) else m).
   Proof.
     unfold transpose_neqkey, Equal; intros.
     unfold honest_perm_filter_fn.
@@ -222,9 +198,9 @@ Section CleanKeys.
 
   Lemma clean_key_permissions_inv :
     forall k_id k ks,
-      clean_key_permissions ks $? k_id = Some k
+      clean_key_permissions honestk ks $? k_id = Some k
       -> ks $? k_id = Some k
-      /\ honest_perm_filter_fn k_id k = true.
+      /\ honest_perm_filter_fn honestk k_id k = true.
   Proof.
     unfold clean_key_permissions; intros until ks.
     rewrite <- !find_mapsto_iff.
@@ -233,39 +209,39 @@ Section CleanKeys.
 
   Lemma clean_key_permissions_inv' :
     forall k_id k ks,
-      clean_key_permissions ks $? k_id = None
+      clean_key_permissions honestk ks $? k_id = None
       -> ks $? k_id = Some k
-      -> honest_perm_filter_fn k_id k = false.
+      -> honest_perm_filter_fn honestk k_id k = false.
   Proof.
     induction ks using P.map_induction_bis; intros; Equal_eq; clean_map_lookups; eauto.
 
     destruct (x ==n k_id); subst; clean_map_lookups; eauto.
     - unfold clean_key_permissions,filter in H0; rewrite fold_add in H0; eauto.
-      cases (honest_perm_filter_fn k_id k); clean_map_lookups; try discriminate; trivial.
+      cases (honest_perm_filter_fn honestk k_id k); clean_map_lookups; try discriminate; trivial.
     - eapply IHks; eauto.
       unfold clean_key_permissions, filter in H0.
       rewrite fold_add in H0; eauto.
-      cases (honest_perm_filter_fn x e); eauto.
+      cases (honest_perm_filter_fn honestk x e); eauto.
       clean_map_lookups; eauto.
   Qed.
 
   Lemma clean_key_permissions_adds_no_permissions :
     forall k_id ks,
         ks $? k_id = None
-      -> clean_key_permissions ks $? k_id = None.
+      -> clean_key_permissions honestk ks $? k_id = None.
   Proof.
     induction ks using P.map_induction_bis; intros; Equal_eq; eauto.
     unfold clean_key_permissions, filter; rewrite fold_add; eauto.
     destruct (x ==n k_id); subst; clean_map_lookups.
-    destruct (honest_perm_filter_fn x e); eauto.
+    destruct (honest_perm_filter_fn honestk x e); eauto.
     clean_map_lookups; eauto.
   Qed.
 
   Lemma clean_key_permissions_keeps_honest_permission :
     forall k_id k ks,
         ks $? k_id = Some k
-      -> honest_perm_filter_fn k_id k = true
-      -> clean_key_permissions ks $? k_id = Some k.
+      -> honest_perm_filter_fn honestk k_id k = true
+      -> clean_key_permissions honestk ks $? k_id = Some k.
   Proof.
     unfold clean_key_permissions; intros.
     rewrite <- !find_mapsto_iff.
@@ -276,14 +252,14 @@ Section CleanKeys.
   Lemma clean_key_permissions_drops_dishonest_permission :
     forall k_id k ks,
         ks $? k_id = Some k
-      -> honest_perm_filter_fn k_id k = false
-      -> clean_key_permissions ks $? k_id = None.
+      -> honest_perm_filter_fn honestk k_id k = false
+      -> clean_key_permissions honestk ks $? k_id = None.
   Proof.
     unfold clean_key_permissions; intros.
     rewrite <- not_find_in_iff.
     unfold not; intros.
     rewrite in_find_iff in H1.
-    cases (filter honest_perm_filter_fn ks $? k_id); try contradiction.
+    cases (filter (honest_perm_filter_fn honestk) ks $? k_id); try contradiction.
     rewrite <- find_mapsto_iff in Heq.
     rewrite filter_iff in Heq; eauto.
     split_ands.
@@ -294,11 +270,11 @@ Section CleanKeys.
 
   Lemma clean_key_permissions_idempotent :
     forall ks,
-      clean_key_permissions ks = clean_key_permissions (clean_key_permissions ks).
+      clean_key_permissions honestk ks = clean_key_permissions honestk (clean_key_permissions honestk ks).
   Proof.
     intros.
     apply map_eq_Equal; unfold Equal; intros.
-    symmetry; cases (clean_key_permissions ks $? y).
+    symmetry; cases (clean_key_permissions honestk ks $? y).
     - generalize (clean_key_permissions_inv _ _ Heq); intros;
         split_ands; apply clean_key_permissions_keeps_honest_permission; eauto.
     - eapply clean_key_permissions_adds_no_permissions; eauto.
@@ -306,25 +282,25 @@ Section CleanKeys.
 
   Lemma clean_key_permissions_distributes_merge_key_permissions :
     forall perms1 perms2,
-      clean_key_permissions (perms1 $k++ perms2) = clean_key_permissions perms1 $k++ clean_key_permissions perms2.
+      clean_key_permissions honestk (perms1 $k++ perms2) = clean_key_permissions honestk perms1 $k++ clean_key_permissions honestk perms2.
   Proof.
     intros; apply map_eq_Equal; unfold Equal; intros.
-    cases (clean_key_permissions perms1 $? y);
-      cases (clean_key_permissions perms2 $? y);
-      cases (clean_key_permissions (perms1 $k++ perms2) $? y); simplify_key_merges1; eauto;
+    cases (clean_key_permissions honestk perms1 $? y);
+      cases (clean_key_permissions honestk perms2 $? y);
+      cases (clean_key_permissions honestk (perms1 $k++ perms2) $? y); simplify_key_merges1; eauto;
         repeat (
             match goal with
-            | [ H1 : honest_perm_filter_fn ?y _ = true, H2 : honest_perm_filter_fn ?y _ = false |- _ ] =>
+            | [ H1 : honest_perm_filter_fn _ ?y _ = true, H2 : honest_perm_filter_fn _ ?y _ = false |- _ ] =>
               unfold honest_perm_filter_fn in *; cases (honestk $? y); try discriminate
             | [ H : (if ?b then _ else _) = _ |- _ ] => destruct b; try discriminate
-            | [ H : clean_key_permissions _ $? _ = Some _ |- _ ] => apply clean_key_permissions_inv in H
-            | [ H0 : ?perms $? ?y = Some _ , H : clean_key_permissions ?perms $? ?y = None |- _ ] =>
+            | [ H : clean_key_permissions _ _ $? _ = Some _ |- _ ] => apply clean_key_permissions_inv in H
+            | [ H0 : ?perms $? ?y = Some _ , H : clean_key_permissions _ ?perms $? ?y = None |- _ ] =>
               apply (clean_key_permissions_inv' _ _ H) in H0; clear H
             | [ H1 : _ $? ?y = Some _, H2 : perms1 $k++ perms2 $? ?y = None |- _ ] =>
               apply merge_perms_no_disappear_perms in H2; split_ands; contra_map_lookup
-            | [ H0 : ?perms $? ?y = None , H : clean_key_permissions ?perms $? ?y = None |- _ ] =>
+            | [ H0 : ?perms $? ?y = None , H : clean_key_permissions _ ?perms $? ?y = None |- _ ] =>
               simplify_key_merges1; eauto 2
-            | [ H : clean_key_permissions ?perms $? ?y = None |- _ ] =>
+            | [ H : clean_key_permissions _ ?perms $? ?y = None |- _ ] =>
               match goal with
                 | [ H : perms $? y = _ |- _ ] => fail 1
                 | _ => cases (perms $? y)
@@ -336,7 +312,7 @@ Section CleanKeys.
   Lemma clean_honest_key_permissions_distributes :
     forall perms pubk,
       (forall k_id kp, pubk $? k_id = Some kp -> honestk $? k_id = Some true /\ kp = false)
-      -> clean_key_permissions (perms $k++ pubk) = clean_key_permissions perms $k++ pubk.
+      -> clean_key_permissions honestk (perms $k++ pubk) = clean_key_permissions honestk perms $k++ pubk.
   Proof.
     intros.
 
@@ -344,13 +320,13 @@ Section CleanKeys.
     apply map_eq_Equal; unfold Equal; intros.
     cases (pubk $? y).
     - specialize (H _ _ Heq); split_ands; subst.
-      assert (clean_key_permissions pubk $? y = Some false)
+      assert (clean_key_permissions honestk pubk $? y = Some false)
         by (eapply clean_key_permissions_keeps_honest_permission; eauto; unfold honest_perm_filter_fn; context_map_rewrites; trivial).
-      cases (clean_key_permissions perms $? y);
+      cases (clean_key_permissions honestk perms $? y);
         simplify_key_merges; eauto.
-    - assert (clean_key_permissions pubk $? y = None) 
+    - assert (clean_key_permissions honestk pubk $? y = None) 
         by (apply clean_key_permissions_adds_no_permissions; eauto).
-      cases (clean_key_permissions perms $? y);
+      cases (clean_key_permissions honestk perms $? y);
         simplify_key_merges; eauto.
   Qed.
 
